src/basic/FStarC.Options.fsti
@@ -205,6 +205,7 @@ val codegen_libs                : unit    -> ML (list (list string))
 val custard_entries             : unit    -> ML (list string)
 val custard_dump_ir             : unit    -> ML bool
 val custard_dump_specializations: unit    -> ML bool
+val custard_dump_layouts: unit           -> ML bool
 val custard_fuel                : unit    -> ML int
 val custard_max_specializations : unit    -> ML int
 val custard_monomorphize_types  : unit    -> ML bool
